


\ifnumequal{\value{rolldice}}{0}{
  % variables 
  \renewcommand{\vbone}{1}
  \renewcommand{\vbtwo}{2}
}{
  \ifnumequal{\value{rolldice}}{1}{
    % variables 
    \renewcommand{\vbone}{2}
    \renewcommand{\vbtwo}{3}
  }{
    \ifnumequal{\value{rolldice}}{2}{
      % variables 
      \renewcommand{\vbone}{3}
      \renewcommand{\vbtwo}{4}
    }{
      % variables 
      \renewcommand{\vbone}{1}
      \renewcommand{\vbtwo}{3}
    }
  }
}

\SQUARE\vbone\aa
\SQUARE\vbtwo\bb
\SUBTRACT\bb\aa\vbthree

\MULTIPLY\vbone{-1}\vbfour

\question[4] Evaluate the following limit \[ \lim_{x\to -\vbone}\dfrac{x + \vbone}{\sqrt{x^2 + \vbthree} - \vbtwo} \] 

\watchout


\begin{solution}[\halfpage]
  Plugging in $x = -\vbone$ will turn the expression into $\frac{A}{0}$ form. Not good. So, we need to 
  do something to turn it into $\frac{C}{D},\, D\neq 0$ form. Lets try rationalizing 

  \begin{align}
    \lim_{x\to -\vbone}\dfrac{x + \vbone}{\sqrt{x^2 + \vbthree} - \vbtwo} &= 
    \lim_{x\to -\vbone}\dfrac{x + \vbone}{\sqrt{x^2 + \vbthree} - \vbtwo}\times\dfrac{\sqrt{x^2 + \vbthree} + \vbtwo}{\sqrt{x^2 + \vbthree} + \vbtwo}  \\
    &= \lim_{x\to -\vbone}\dfrac{(x + \vbone)\cdot(\sqrt{x^2 + \vbthree} + \vbtwo)}
    {\underbrace{(x^2 + \vbthree) - \bb}_{x^2-\aa = (x-\vbone)\cdot(x+\vbone)}} \\
    &= \lim_{x\to -\vbone}\dfrac{(\sqrt{x^2 + \vbthree} + \vbtwo)}{x-\vbone} = \WRITEFRAC\vbtwo\vbfour
  \end{align}
\end{solution}

