


\ifnumequal{\value{rolldice}}{0}{
  % variables 
  \renewcommand{\vbone}{1}
  \renewcommand{\vbtwo}{2}
  \renewcommand{\vbthree}{4}
  \renewcommand{\vbfour}{6}
}{
  \ifnumequal{\value{rolldice}}{1}{
    % variables 
    \renewcommand{\vbone}{3}
    \renewcommand{\vbtwo}{7}
    \renewcommand{\vbthree}{2}
    \renewcommand{\vbfour}{4}
  }{
    \ifnumequal{\value{rolldice}}{2}{
      % variables 
      \renewcommand{\vbone}{2}
      \renewcommand{\vbtwo}{6}
      \renewcommand{\vbthree}{5}
      \renewcommand{\vbfour}{9}
    }{
      % variables 
      \renewcommand{\vbone}{5}
      \renewcommand{\vbtwo}{4}
      \renewcommand{\vbthree}{3}
      \renewcommand{\vbfour}{7}
    }
  }
}

\SQUARE\vbtwo\tp
\gcalcexpr[0]\tq{\vbfour * \tp}
\ADD\tq\vbthree\tr
\MULTIPLY\vbtwo{2}\ts

\question[3] Given two functions - $f(x)$ and $g(x)$ - find $f'(x)$ given that 
$g(\vbone) = \vbtwo$, $\left.\dfrac{d}{dx} f(x)g(x)\right\vert_{x=\vbone} = \vbthree$ and 
$\dfrac{d}{dx}\left.\dfrac{f(x)}{g(x)}\right\vert_{x=\vbone} = \vbfour$

\watchout

\ifprintanswers
\fi 

\begin{solution}[\halfpage]
	We know that, 
	\begin{align}
		\text{(Product Rule) }\dfrac{d}{dx} f\cdot g &= f'g + g'f \\
		\text{(Quotient Rule) }\dfrac{d}{dx}\dfrac{f}{g} &= \dfrac{gf' - g'f}{g^2}
	\end{align}
	
	And therefore, when $x=\vbone$, the following would hold 
	\begin{align}
		\vbtwo\cdot f' + g'f &= \vbthree \Rightarrow g'f = \vbthree - \vbtwo\cdot f' \\
		\dfrac{\vbtwo\cdot f' - g'f }{\vbtwo^2} &= \vbfour \Rightarrow g'f = \vbtwo\cdot f' - \tq \\
		\Rightarrow \vbthree - \vbtwo\cdot f' &= \vbtwo\cdot f' - \tq \\
		\text{ or } f'(x) &= \WRITEFRAC\tr\ts
	\end{align}
\end{solution}

