

\question Evaluate the limit \[ \lim_{x\to 1}\dfrac{x^{\frac{1}{3}}-1}{x^{\frac{1}{4}}-1}\]

\begin{solution}
  \textbf{Let} $x = z^4$. \textbf{Then} $\lim_{x\to 1} \Longleftrightarrow \lim_{z\to 1}$ and $x^{\frac{1}{3}} = z^{\frac{4}{3}}$. Or, 
  \begin{align}
    \lim_{x\to 1}\dfrac{x^{\frac{1}{3}} - 1}{x^{\frac{1}{4}} - 1} &= 
    \lim_{z\to 1}\dfrac{z^{\frac{4}{3}} - 1}{z - 1} \\
    &=\lim_{z\to 1}\dfrac{z^{\frac{4}{3}} - z^{\frac{1}{3}} + z^{\frac{1}{3}} - 1}{z - 1} \\
    &= \lim_{z\to 1}\dfrac{z^{\frac{1}{3}}\cdot (z-1) + (z^{\frac{1}{3}} - 1)}{z-1} \\
    &= \underbrace{\lim_{z\to 1}z^{\frac{1}{3}}}_{= 1} + 
    \underbrace{\lim_{z\to 1}\dfrac{z^{\frac{1}{3}} - 1}{z-1}}_{\texttt{Unknown}}
  \end{align}
  
  As before, let $z = w^3$ so that $\lim_{z\to 1}\Longleftrightarrow\lim_{w\to 1}$ and, 
  \begin{align}
    \lim_{z\to 1}\dfrac{z^{\frac{1}{3}}-1}{z-1} &= \lim_{w\to 1}\dfrac{w-1}{w^3-1} \\
    &= \lim_{w\to 1}\dfrac{w-1}{(w-1)\cdot (w^2+w+1)} = \dfrac{1}{3}
  \end{align}
  Our final answer is therefore $= 1+\frac{1}{3} = \dfrac{4}{3}$
\end{solution}
