

\printrubric

\question[4] Find an expression for the sum of the first $n$ terms of the series 
$\dfrac{1}{1\cdot 2\cdot 3} + \dfrac{1}{2\cdot 3\cdot 4} + \dfrac{1}{3\cdot 4\cdot 5} + \ldots$


\ifprintanswers
\fi 

\begin{solution}[\fullpage]
	Each term in the series is of the form $a_n = \dfrac{1}{n\cdot(n+1)\cdot(n+2)}$. And therefore,
	\begin{align}
		S_n &= \sum_{k=1}^{n}\dfrac{1}{k\cdot(k+1)\cdot(k+2)} 
		= \sum_{k=1}^{n}\dfrac{k+1-k}{k\cdot(k+1)\cdot(k+2)} \\
		&= \sum_{k=1}^{n}\dfrac{1}{k\cdot(k+2)} - \sum_{k=1}^{n}\dfrac{1}{(k+1)\cdot(k+2)} \\
		&= \dfrac{1}{2}\sum_{k=1}^{n}\dfrac{k+2-k}{(k+2)\cdot k} - \sum_{k=1}^{n}\dfrac{k+1-k}{(k+1)\cdot k} \\
		&= \dfrac{1}{2}\left[\sum_{k=1}^{n}\dfrac{1}{k} - \sum_{k=1}^{n}\dfrac{1}{k+2} \right] 
		- \left[ \sum_{k=1}^{n}\dfrac{1}{k} - \sum_{k=1}^{n}\dfrac{1}{k+1} \right] \\
		&= \dfrac{1}{2}\left[\left(1 + \frac{1}{2} + \frac{1}{3} + \ldots + \frac{1}{n} \right) 
		- \left( \frac{1}{3} + \frac{1}{4} + \ldots + \frac{1}{n} + \frac{1}{n+1} + \frac{1}{n+2}\right) 
		\right] \nonumber \\
		&- \left[\left( \frac{1}{2} + \frac{1}{3} + \ldots + \frac{1}{n+1}\right) 
		- \left( \frac{1}{3} + \frac{1}{4} + \ldots + \frac{1}{n+1} + \frac{1}{n+2} \right) \right]  \\
		&= \dfrac{1}{2}\left[ \dfrac{3}{2} - \dfrac{1}{n+1} - \dfrac{1}{n+2}\right] 
		- \left[\dfrac{1}{2} - \dfrac{1}{n+2} \right] \\
		&= \dfrac{1}{4} - \dfrac{1}{2}\left( \dfrac{1}{n+1} - \dfrac{1}{n+2}\right) \\
		&= \dfrac{1}{4} - \dfrac{1}{2}\cdot\dfrac{1}{(n+1)\cdot(n+2)}
	\end{align}
\end{solution}

