

\question[3] Three numbers form an arithmetic progression. The sum of the numbers is equal to 3 and 
the sum of their cubes is equal to 4. Find the numbers


\ifprintanswers
  % stuff to be shown only in the answer key - like explanatory margin figures
  \marginnote[3cm] {Setting $a=1$ in $(2)$}
\fi 

\begin{solution}[\halfpage]
  Let the numbers be $a-d$, $a$ and $a+d$. And here is what we know 
  \begin{align}
     (a-d) + a + (a + d) &= 3 \Rightarrow a = 1 \\
     (1-d)^3 + 1^3 + (1+d)^3 &= 4 \\
     \underbrace{(1-3d+3d^2-d^3)}_{(1-d)^3} + 1 +
            \underbrace{(1+3d+3d^2+d^3)}_{(1+d)^3} &= 4 \\
     \Rightarrow d &= \dfrac{1}{\sqrt{6}}
  \end{align}
  
  The numbers, therefore, are $\left(1-\frac{1}{\sqrt{6}}\right)$, $1$ and 
  $\left(1+\frac{1}{\sqrt{6}}\right)$
\end{solution}
