

\question[2]  Prove the following  
\[ (1+\cot A+\tan A)(\sin A-\cos A)=(\sin A\tan A-\cot A\cos A) \]

\begin{solution}[\halfpage]
  \begin{align}
     &(1+\cot A+\tan A)(\sin A-\cos A) = \nonumber\\
		 &\left( 1+\dfrac{\cos A}{\sin A} + \dfrac{\sin A}{\cos A}\right)\cdot (\sin A - \cos A) \\
		 &= \left( \sin A + \sin A\cdot\dfrac{\cos A}{\sin A} + \sin A\cdot\dfrac{\sin A}{\cos A}\right) \nonumber\\
		 &-\cos A - \cos A\cdot\dfrac{\cos A}{\sin A} - \cos A\cdot\dfrac{\sin A}{\cos A} \\
		 &= \sin A + \cos A + \sin A\cdot\tan A - \cos A - \cos A\cdot\cot A - \sin A \\
		 &= \sin A\cdot\tan A - \cos A\cdot \cot A
  \end{align}

\end{solution}
