
<<<<<<< HEAD


\ifnumequal{\value{rolldice}}{0}{
  \renewcommand{\vbone}{}
  \renewcommand{\vbtwo}{}
  \renewcommand{\vbthree}{}
  \renewcommand{\vbfour}{}
  \renewcommand{\vbfive}{}
  \renewcommand{\vbsix}{}
  \renewcommand{\vbseven}{}
  \renewcommand{\vbeight}{}
  \renewcommand{\vbnine}{}
  \renewcommand{\vbten}{}
}{
  \ifnumequal{\value{rolldice}}{1}{
    \renewcommand{\vbone}{}
    \renewcommand{\vbtwo}{}
    \renewcommand{\vbthree}{}
    \renewcommand{\vbfour}{}
    \renewcommand{\vbfive}{}
    \renewcommand{\vbsix}{}
    \renewcommand{\vbseven}{}
    \renewcommand{\vbeight}{}
    \renewcommand{\vbnine}{}
    \renewcommand{\vbten}{}
  }{
    \ifnumequal{\value{rolldice}}{2}{
      \renewcommand{\vbone}{}
      \renewcommand{\vbtwo}{}
      \renewcommand{\vbthree}{}
      \renewcommand{\vbfour}{}
      \renewcommand{\vbfive}{}
      \renewcommand{\vbsix}{}
      \renewcommand{\vbseven}{}
      \renewcommand{\vbeight}{}
      \renewcommand{\vbnine}{}
      \renewcommand{\vbten}{}
    }{
      \renewcommand{\vbone}{}
      \renewcommand{\vbtwo}{}
      \renewcommand{\vbthree}{}
      \renewcommand{\vbfour}{}
      \renewcommand{\vbfive}{}
      \renewcommand{\vbsix}{}
      \renewcommand{\vbseven}{}
      \renewcommand{\vbeight}{}
      \renewcommand{\vbnine}{}
      \renewcommand{\vbten}{}
=======

\ifnumequal{\value{rolldice}}{0}{
  % variables 
  \renewcommand{\vbone}{7}
}{
  \ifnumequal{\value{rolldice}}{1}{
    % variables 
    \renewcommand{\vbone}{3}
  }{
    \ifnumequal{\value{rolldice}}{2}{
      % variables 
      \renewcommand{\vbone}{4}
    }{
      % variables 
      \renewcommand{\vbone}{5}
>>>>>>> b522d18472a6ac8941d0010c7d5e3e533e79be60
    }
  }
}

<<<<<<< HEAD
\question[1] Find $\lim_{x\to 1}\frac{\left(\sqrt{(x^2-1)}+ \sqrt{x-1}\right)}{\sqrt{x^2-1}}$ 
=======
\SQUARE\vbone\vbtwo
\MULTIPLY\vbone{2}\vbthree
>>>>>>> b522d18472a6ac8941d0010c7d5e3e533e79be60

\question[1] Evaluate the following limit \[ \lim_{x\to\vbone}\dfrac{\sqrt{x^2 -\vbtwo} + \sqrt{x-\vbone}}{\sqrt{x^2-\vbtwo}}\]

\watchout

<<<<<<< HEAD
\ifprintanswers
  \begin{marginfigure}
    \figinit{pt}
      \figpt 100:(0,0)
      \figpt 101:(0,0)
    \figdrawbegin{}
      \figdrawline [100,101]
    \figdrawend
    \figvisu{\figBoxA}{}{%
    }
    \centerline{\box\figBoxA}
  \end{marginfigure}
\fi 

\begin{solution}[\mcq]
Given limit is of the form : $\frac{0}{0}$\\
By simply expanding the given expression we get can get this into determinate form. 
Hence we do  not to apply the L-Hospital rule.
\begin{align}
&\Rightarrow \lim_{x\to 1}\frac{\left(\sqrt{(x^2-1)}+ \sqrt{x-1}\right)} {\sqrt{x^2-1}} \\
&= \lim_{x\to 1}\frac{\sqrt{(x-1)(x+1)} + \sqrt{x-1}}{\sqrt{(x-1)(x+1)}} \\
&= \lim_{x\to 1}\frac{\sqrt{(x+1)} + 1 }{\sqrt{(x+1)}} \\
&= \dfrac{\sqrt{2}+1}{\sqrt{2}} 
\end{align}
=======
\begin{solution}[\mcq]
  \begin{align}
    \lim_{x\to\vbone}\dfrac{\sqrt{x^2-\vbtwo} + \sqrt{x-\vbone}}{\sqrt{x^2-\vbtwo}} &= 
    \lim_{x\to\vbone}\dfrac{\sqrt{x-\vbone}\cdot (\sqrt{x+\vbone} + 1)}{\sqrt{x-\vbone}\cdot\sqrt{x + \vbone}} \\
    &= \lim_{x\to\vbone}\dfrac{\sqrt{x+\vbone} + 1}{\sqrt{x + \vbone}} 
    = 1 + \frac{1}{\sqrt\vbthree}
  \end{align}
>>>>>>> b522d18472a6ac8941d0010c7d5e3e533e79be60
\end{solution}

