

\question[3] Find an expression for the sum of the first $n$ terms of 
$\dfrac{1}{1\cdot 4} + \dfrac{1}{4\cdot 7} + \ldots + \dfrac{1}{(3n-2)\cdot(3n+1)} + \ldots$


\ifprintanswers
\fi 

\begin{solution}[\halfpage]
	\begin{align}
		S_n &= \sum_{k=1}^{n}\dfrac{1}{(3n-2)\cdot(3n+1)} = 
		\sum_{k=1}^{n}\dfrac{1}{3}\cdot\dfrac{(3n+1) - (3n-2)}{(3n-2)\cdot(3n+1)} \\
		&= \dfrac{1}{3}\left[ \sum_{k=1}^{n}\dfrac{1}{3n-2} - \sum_{k=1}^{n}\dfrac{1}{3n+1}\right]
	\end{align}
	Now, $3n-2 = 3k + 1$ if $n = k + 1$. Which means, that every term \textit{after} the first
	term in the first summand can be found in the second summand - and, more importantly - will 
	cancel itself out. In other words,
	
	\begin{align}
		S_n &= \dfrac{1}{3}\cdot\left[\left( 1+\frac{1}{4}+\ldots +\frac{1}{3n-2}\right)
		- \left( \frac{1}{4} + \ldots + \frac{1}{3n-2} + \frac{1}{3n+1}\right) \right] \\
		&= \dfrac{1}{3}\cdot\left( 1-\dfrac{1}{3n+1}\right) = \dfrac{n}{3n+1}
	\end{align}
\end{solution}
