


\ifnumequal{\value{rolldice}}{0}{
  % variables 
}{
  \ifnumequal{\value{rolldice}}{1}{
    % variables 
  }{
    \ifnumequal{\value{rolldice}}{2}{
      % variables 
    }{
      % variables 
    }
  }
}

\question Consider the curve given by $xy^2-x^3y=6$.



\ifprintanswers
  % stuff to be shown only in the answer key - like explanatory margin figures
  \begin{marginfigure}
    \figinit{pt}
      \figpt 100:(0,0)
      \figpt 101:(0,0)
    \figdrawbegin{}
      \figdrawline [100,101]
    \figdrawend
    \figvisu{\figBoxA}{}{%
    }
    \centerline{\box\figBoxA}
  \end{marginfigure}
\fi 

\begin{parts}
  \part[2] Show that $\dydx = \dfrac{3x^2y-y^2}{2xy-x^3}$.

\begin{solution}[\mcq]
    \begin{align}
                  &xy^2-x^3y=6 \\
      \Rightarrow &x(2y)\dydx+y^2\cdot 1-\left[x^3\dydx +y(3x^2)\right]=0 \\
      \Rightarrow &\dydx = \dfrac{3x^2y-y^2}{2xy-x^3}    
    \end{align}
  \end{solution}

  \part[3] Find all the points on the curve whose \textit{x-coordinate} is $1$ and 
  write an equation for the tangent line at each of these points.

\begin{solution}[\mcq]
    Substitute $x=1$ in the equation of the curve,
    \begin{align}
      &y^2-y=6 \Rightarrow y=3 \text{ or } y=-2
    \end{align}
    To find the equation for the tangent line we need the $derivative$ (slope)
    of the function at these two points.
    \begin{align}
      \dydx {\displaystyle\vert}_{(1,3)} &=0 \Rightarrow y=3\\ 
      \dydx {\displaystyle\vert}_{(1,-2)}&=2 \Rightarrow y+2=2(x-1) \\
                                         &\quad\quad\Rightarrow y=2x-4)
    \end{align}
  \end{solution}

  \part[3] Find the \textit{x-coordinate} of each point on the curve where the tangent
  line is vertical.
\begin{solution}[\mcq]
    The tangent is vertical when $\dfrac{\ud x}{\ud y}$ is $0$. Therefore,
    \begin{align}
                  &\dfrac{2xy-x^3}{3x^2y-y^2}=0 \\
      \Rightarrow &2xy-x^3=0 \textit{ (and $3x^2y-y^2\neq 0$)} \\
      \Rightarrow &2xy-x^3=0 \Rightarrow x(2y-x^2)=0 \\
      \Rightarrow &x=0 \text{ or } y=\dfrac{1}{2}x^2
    \end{align}
    $x=0$ rejected, therefore using $y =\dfrac{1}{2}x^2$
    \begin{align}
                  &\dfrac{1}{4}x^5-\dfrac{1}{2}x^5=6 \\
      \Rightarrow &x^5 =-24 \Rightarrow x=\sqrt[5]{-24}
    \end{align}
  \end{solution}
\end{parts}

