


\ifnumequal{\value{rolldice}}{0}{
  \renewcommand{\vbone}{57}
}{
  \ifnumequal{\value{rolldice}}{1}{
    \renewcommand{\vbone}{63}
  }{
    \ifnumequal{\value{rolldice}}{2}{
      \renewcommand{\vbone}{101}
    }{
      \renewcommand{\vbone}{79}
    }
  }
}

\SUBTRACT\vbone{1}\vbtwo

\question[3] Differentiate $y=\cos^2(x^{\vbone})$ with respect to $x$

\insertQR{}

\watchout

\ifprintanswers
\fi 

\begin{solution}[\halfpage]
  If $z = \cos(x^{\vbone})$, then $y = z^2$ and \textbf{chain-rule} tells us that 
  \begin{align}
    \dydx &= \dfrac{\mathrm{d}}{\mathrm{d}z}z^2\cdot\dydx[z] \\
    &= 2z\cdot\dydx[\cos(x^{\vbone})] \\
    &= \underbrace{(2\cos x^{\vbone})\cdot(-\sin x^{\vbone})}_{2\sin\theta\cos\theta = \sin 2\theta}\cdot\vbone\cdot x^{\vbtwo} \\
    &= -\vbone\cdot x^{\vbtwo}\cdot\sin (2x^{\vbone})
  \end{align}
  \textbf{Alternatively,} one could also say that given $\cos^2 x = \dfrac{\cos 2x + 1}{2}$,
  \begin{align}
    \dydx &= \dydx[\left( \dfrac{\cos 2x^{\vbone} + 1}{2}\right)] 
    = \dfrac{1}{2}\dydx[\cos 2x^{\vbone}] \\
    &= \dfrac{1}{2}\cdot (-\sin 2x^{\vbone} )\cdot\dydx[2x^{\vbone}] \\
    &= \dfrac{1}{2}\cdot (-\sin 2x^{\vbone} )\cdot (2\cdot\vbone\cdot x^{\vbtwo}) \\
    &= -\vbone\cdot x^{\vbtwo}\cdot\sin (2x^{\vbone})
  \end{align}
\end{solution}

