

\question[3] Prove that $\tan\left(\dfrac{\pi}{4} + \theta\right) + 
\tan\left(\dfrac{\pi}{4} - \theta\right) = 2\sec 2\theta$


\ifprintanswers
\fi 

\begin{solution}[\halfpage]
	\begin{align}
		\tan\left(\dfrac{\pi}{4} + \theta\right) &+ \tan\left(\dfrac{\pi}{4} - \theta\right) = 
		\eTanOfSum{\frac{\pi}{4}}{\theta} + \eTanOfDiff{\frac{\pi}{4}}{\theta} \\
		&= \dfrac{(1+\tan\theta)^2 + (1-\tan\theta)^2}{1-\tan^2\theta} \\
		&= \dfrac{2\cdot(1 + \tan^2\theta)}{1-\tan^2\theta} = \dfrac{2\sec^2\theta}{1-\tan^2\theta} \\
    &= \dfrac{2}{\underbrace{\cos^2\theta - \sin^2\theta}_{ = \cos 2\theta}} = 2\sec 2\theta
	\end{align}
\end{solution}
