

\question[3] Find the sum of the first $n$ terms of the series $1^3 + 3^3 + 5^3 + 7^3 \ldots$ 


\ifprintanswers
	\marginnote[3cm]{ $(a-b)^3 = a^3-3a^2b + 3ab^2 - b^3$ }
\fi 

\begin{solution}[\halfpage]
	If $a_n$ be the $n^{th}$ term of the series, then we can see that $a_n = (2k-1)^3,\, k \geq 1$.
	Hence, the sum of the first $n$ terms would be 
	\begin{align}
		S_n &= \sum_{k=1}^{n}(2k-1)^3 = \sum_{k=1}^{n}8k^3 - 
		\sum_{k=1}^{n}3\cdot 4k^2 + \sum_{k=1}^{n}3\cdot 2k - \sum_{k=1}^{n} 1 \\
		&= 8\cdot\eSumOfCubes{n} - 12\cdot\eSumOfSquares{n} + 6\cdot\eSumOfN{n} - n \\
		&= n\cdot(n+1)\cdot[2n\cdot(n+1) - 2\cdot(2n+1) + 3 ] - n \\
		&= n\cdot(n+1)\cdot(2n^2-2n+1) - n \\
    &= n\cdot\left[ (n+1)\cdot(2n^2-2n+1) - 1\right] \\
    &= n\cdot\left( 2n^3-2n^2+n + 2n^2-2n + 1 -1\right) = n\cdot(2n^3-n) \\
    &= n^2\cdot(2n^2-1)
	\end{align}
\end{solution}
 
