

\ifnumequal{\value{rolldice}}{0}{
  % variables 
  \renewcommand{\vbone}{2}
}{
  \ifnumequal{\value{rolldice}}{1}{
    % variables 
    \renewcommand{\vbone}{4}
  }{
    \ifnumequal{\value{rolldice}}{2}{
      % variables 
      \renewcommand{\vbone}{3}
    }{
      % variables 
      \renewcommand{\vbone}{5}
    }
  }
}

\ADD\vbone{1}\vbtwo
\ADD\vbone{2}\vbthree
\ADD\vbone{3}\vbfour
\ADD\vbone{4}\vbfive

\question[3] Find an expression for the sum of the first $n$ terms of the series 
$\dfrac{1}{\vbtwo\cdot\vbthree} + \dfrac{1}{\vbthree\cdot\vbfour} + \dfrac{1}{\vbfour\cdot\vbfive}\ldots$


\ifprintanswers
\fi 

\begin{solution}[\halfpage]
	 $a_n = \dfrac{1}{(n+\vbone)\cdot(n+\vbtwo)},\, n \geq 1, n\in\mathbb{N}$ in the above series. 
	 The sum of the first $n$ terms, therefore, is given by 
	 \begin{align}
	 	S_n &= \sum_{k=1}^{n}\dfrac{1}{(k+\vbone)\cdot(k+\vbtwo)} =
	 	  \sum_{k=1}^{n}\dfrac{k+\vbtwo - (k+\vbone)}{(k+\vbone)\cdot(k+\vbtwo)} \\
	 	&= \sum_{k=1}^{n}\dfrac{1}{k+\vbone} - \sum_{k=1}^{n}\dfrac{1}{k+\vbtwo} \\
	 	&= \left( \frac{1}{\vbtwo} + \frac{1}{\vbthree} + \frac{1}{\vbfour} + \ldots + \frac{1}{n+\vbone}\right) - 
	 	\left( \frac{1}{\vbthree} + \frac{1}{\vbfour} + \ldots + \frac{1}{n+\vbone} + \frac{1}{n+\vbtwo}\right) \\
	 	&= \dfrac{1}{\vbtwo} - \dfrac{1}{n+\vbtwo} = \dfrac{n}{\vbtwo\cdot(n+\vbtwo)}
	 \end{align}
\end{solution}
