

\question[4] Find an expression for the sum of the first $n$ terms of the series 
$1\cdot 2\cdot 5 + 2\cdot 3\cdot 6 + 3\cdot 4\cdot 7 + 4\cdot 5\cdot 8 + \ldots $


\ifprintanswers
\fi 

\begin{solution}[\halfpage]
	If you look for a pattern in the terms in the above series, then you will soon realize
	that each term is of the form $a_n = n\cdot(n+1)\cdot(n+4)$. And therefore, the sum of 
	the first $n$ terms is given by
	\begin{align}
		S_n &= \sum_{k=1}^{n}\lbrace n\cdot(n+1)\cdot(n+4)\rbrace \\
		&= \sum_{k=1}^{n}(n^3+5n^2+4n) = \sum_{k=1}^{n}n^3 + 5\cdot\sum_{k=1}^{n}n^2 + 4\cdot\sum_{k=1}^{n}n \\
		&= \eSumOfCubes{n} + 5\cdot\eSumOfSquares{n} + 4\cdot\eSumOfN{n} \\
		&= \dfrac{n\cdot(n+1)}{2}\cdot\left[ \dfrac{n\cdot(n+1)}{2} + \dfrac{5}{3}\cdot(2n+1) + 4\right] \\
		&= \dfrac{n\cdot(n+1)}{12}\cdot\lbrace 3n\cdot(n+1) + 10\cdot(2n+1) + 24\rbrace \\
		&= \dfrac{n\cdot(n+1)}{12}\cdot(3n^2 + 23n + 34)
	\end{align}
\end{solution}
