

\question[3]  The angle of elevation of the top of a tower from a point $A$
due south of it is $\alpha$ and $\beta$ from a point $B$ due east of it. If $AB=d$, 
then prove that the height of the tower - $H$ - is equal to 
$\dfrac{d}{\sqrt{\cot^2\alpha + \cot^2\beta}}$


\ifprintanswers
  % stuff to be shown only in the answer key - like explanatory margin figures
	\begin{marginfigure}
		\figinit{pt}
    \figpt 0:$\texttt{Tower(O)}$ (10,0)
    \figpt 1:$A$ (10,-40)
    \figpt 2:$B$ (80,0)
    \figvectP 10 [1,2]
    \figpttra 3:$d$= 1/0.5, 10/
		\figdrawbegin{}
			\figdrawline[0,1,2,0]
		\figdrawend
		\figvisu{\figBoxA}{Top-view}{
      \figwriten 0:(5)
      \figwrites 1:(5)
      \figwritee 2:(5)
      \figwritese 3:(5)
    }
		\centerline{\box\figBoxA}
	\end{marginfigure}

  \begin{marginfigure}[0.5cm]
    \figinit{pt}
      \figpt 0:$A$ (10,0)
      \figpt 1:$\texttt{Tower(O)}$ (80,0)
      \figpt 2: (80,50)
      \figpt 3:$\alpha$ (30,3)

    \figdrawbegin{}
      \figdrawline [0,1,2,0]
      \figdrawarccircP 0;13 [1,2]
    \figdrawend
    \figvisu{\figBoxA}{South-side}{
      \figwritesw 0:(5)
      \figwritee 1:(5)
      \figwriten 3:(0)
    }
		\centerline{\box\figBoxA}
  \end{marginfigure}

  \begin{marginfigure}[0.5cm]
    \figinit{pt}
      \figpt 0:$\texttt{Tower(O)}$ (10,0)
      \figpt 1:$B$ (80,0)
      \figpt 2: (10,50)
      \figpt 3:$\beta$ (60,3)

    \figdrawbegin{}
      \figdrawline [0,1,2,0]
      \figdrawarccircP 1;13 [2,0]
    \figdrawend
    \figvisu{\figBoxA}{East-side}{
      \figwrites 0:(5)
      \figwritee 1:(5)
      \figwriten 3:(0)
    }
		\centerline{\box\figBoxA}
  \end{marginfigure}
\fi  

\begin{solution}[\fullpage]
	From the adjoining figures, we know the following:
	\begin{align}
		\text{Top-view} &: OA^2 + OB^2 = d^2 \\
		\text{South-side} &: OX = H = OA \times\tan\alpha \Rightarrow OA = H\cdot\cot\alpha \\
		\text{East-side} &: OX = H = OB \times\tan\beta \Rightarrow OB = H\cdot\cot\beta
	\end{align}
	
	Substituting (2) and (3) in (1), we get
	\begin{align}
		(H\cdot\cot\alpha)^2 + (H\cdot\cot\beta)^2 &= d^2 \\
		\Rightarrow H^2 &= \dfrac{d^2}{\cot^2\alpha + \cot^2\beta} \\
		\Rightarrow H &= \dfrac{d}{\sqrt{\cot^2\alpha + \cot^2\beta}}
	\end{align}
\end{solution}
