
\question Prove - or disprove - the following proposition using mathematical induction 
\[ x^{2n} - 1 \text{ is divisible by } x + 1,\, x\neq -1 \]

\insertQR{}

\begin{solution}
  \textbf{If} $x^{2n}-1$ is divisible by $x-1$, \textbf{then} for the proposition to be 
  true, it must also hold for $n+1$. 

  \begin{align}
    \dfrac{x^{2\cdot(n+1)}-1}{x+1} &= \overbrace{\dfrac{x^2\cdot x^{2n} - x^2 + x^2 - 1}{x+1}}^{\text{adding and subtracting $x^2$}} \\
    &= \dfrac{x^2\cdot (x^{2n} - 1)}{x+1} + \underbrace{x-1}_{\frac{x^2-1}{x+1}}
  \end{align}

  As $(x^{2n}-1)$ is \textbf{assumed to be} divisible by $x+1$, 
  \[ \dfrac{x^{2\cdot (n+1)} - 1}{x + 1} = x^2\cdot\underbrace{\dfrac{x^{2n}-1}{x+1}}_{Q(x)} + (x-1) = P(x)\]
  where $Q(x)$ and $P(x)$ are some polynomials in $x\implies$ divisibility.

  Moreover, for $n=1$, we can see that $x^{2\cdot 1}-1$ is divisible by $x+1$. Which means, 
  the same would also be true for $n=2,3,4,\ldots,\infty$. Hence proved.
\end{solution}
