
% \noprintanswers
% \setcounter{rolldice}{0}
% \printrubric

\question Evaluate $\limit{x}{\infty}\left( 1-\frac{1}{x}\right)^x$ using L'Hospital's Rule.
\texttt{Hint:} $e^{\ln X} = X$. And therefore, $\limit{x}{\infty}f(x) = \limit{x}{\infty}e^{\ln f(x)} 
= e^{\limit{x}{\infty}\ln f(x)}$

\insertQR{}

\ifprintanswers
\fi 

\begin{solution}
  You have been given a hint. So, lets use it to re-write the original limit 
  \begin{align}
    \limit{x}{\infty}\left( 1-\frac{1}{x} \right)^x &= e^{\limit{x}{\infty}\ln\left( 1-\frac{1}{x} \right)^x}
  \end{align}
  Now, 
  \begin{align}
    \limit{x}{\infty}\ln\left( 1-\frac{1}{x} \right)^x &= \limit{x}{\infty}x\cdot\ln\left( 1-\frac{1}{x}\right) \\
    &= \limit{x}{\infty}\dfrac{\ln\left(1-\frac{1}{x}\right)}{\frac{1}{x}}
  \end{align}
  Applying L'Hospital's Rule to the last equation, we get 
  \begin{align}
    \limit{x}{\infty}\dfrac{\ln\left(1-\frac{1}{x}\right)}{\frac{1}{x}} 
    &= \limit{x}{\infty}\dfrac{\frac{1}{\left( 1-\frac{1}{x}\right)}\cdot\frac{1}{x^2}}{-\frac{1}{x^2}}
    &= \limit{x}{\infty}-\dfrac{1}{\left( 1-\frac{1}{x}\right)} = -1
  \end{align}
  Back to (1), and we get 
  \begin{align}
    \limit{x}{\infty}\left( 1-\frac{1}{x} \right)^x 
    &= e^{\limit{x}{\infty}\ln\left( 1-\frac{1}{x} \right)^x} = e^{-1} = \dfrac{1}{e}
  \end{align}
\end{solution}

