
\question Prove - or disprove - the following proposition
\[ x^n - y^n \text{ is divisible by } x - y,\, x\neq y\]

\insertQR{}

\begin{solution}
  Let $\frac{y}{x}=k$ so that $x-y = x\cdot(1-k)$ and $x^n-y^n=x^n\cdot (1-k^n)$.

  Now, \textbf{if} $x^n-y^n$ is divisible by $x-y$, then 
  \begin{align}
    \dfrac{x^n-y^n}{x-y} &= \dfrac{x^n\cdot(1-k^n)}{x(1-k)} = \dfrac{x^{n-1}\cdot(1-k^n)}{1-k} = Q(x)
  \end{align}
  , where $Q(x) = $ some polynomial in $x$. 
  
  In other words, if $Q(x)$ exists, then  $1-k^n$ is divisible by $1-k$. And that in turn implies 
  that $x^n-y^n$ is divisible by $x-y$.

  Hence, if we can prove that 
  \[ 1-k^{n+1} \text{ is divisible by } 1-k \]
  then we would have proven 
  \[ \dfrac{x^{n+1} - y^{n+1}}{x-y} = \dfrac{x^n\cdot(1-k^{n+1})}{1-k} = P(x)\implies\text{ divisiblity }\]
  where $P(x)$ is another polynomial - like $Q(x)$. Now, 
  \begin{align}
    \dfrac{1-k^{n+1}}{1-k} &= \dfrac{1-k + k - k^{n+1}}{1-k} \\
      &= 1 + \dfrac{k\cdot (1-k^n)}{1-k}
  \end{align}

  And \textbf{ because we assumed } that $1-k^n$ is divisible by $1-k$, \textbf{ then so would } $1-k^{n+1}$ be. 
  \textbf{Morever,} we can see that $1-k^n$ is divisible by $1-k$ for $n=1\implies 1-k^n$ is also 
  divisible by $1-k$ for $n=2,3,4,\ldots,\infty$. 

  And as $k=\frac{y}{x}$, the fact that $1-k^n$ is divisible by $1-k\implies x^n-y^n$ is divisible by $x-y$.
\end{solution}

