

\ifnumequal{\value{rolldice}}{0}{
  \renewcommand{\vbone}{8}
  \renewcommand{\vbtwo}{4}
  \renewcommand{\vbthree}{16}
  \renewcommand{\vbfour}{64}
  \renewcommand{\vbfive}{48}
}{
  \ifnumequal{\value{rolldice}}{1}{
    \renewcommand{\vbone}{10}
    \renewcommand{\vbtwo}{5}
    \renewcommand{\vbthree}{20}
    \renewcommand{\vbfour}{100}
    \renewcommand{\vbfive}{60}
  }{
    \ifnumequal{\value{rolldice}}{2}{
      \renewcommand{\vbone}{6}
      \renewcommand{\vbtwo}{3}
      \renewcommand{\vbthree}{12}
      \renewcommand{\vbfour}{36}
      \renewcommand{\vbfive}{36}
    }{
      \renewcommand{\vbone}{12}
      \renewcommand{\vbtwo}{6}
      \renewcommand{\vbthree}{24}
      \renewcommand{\vbfour}{144}
      \renewcommand{\vbfive}{72}
    }
  }
}

\question[2] Break up the number $\vbone$ into two summands such that the sum of their cubes
is the least possible

\watchout 

\ifprintanswers
  % stuff to be shown only in the answer key - like explanatory margin figures
\fi

\begin{solution}[\halfpage]
   Basically, we have to minimize $y = x^3 + (\vbone-x)^3$
   \begin{align}
      y &= x^3 + (\vbone -x)^3, \text{ then } \\
      \dydx &= 3x^2 - 3(\vbone - x)^2 \text{ and } \\
      \dnydxn{2} &= 6x + 6(\vbone-x)
   \end{align}
   
   Now, 
   \begin{align}
      \dydx &= 0 \text { when } 3x^2 - 3(\vbone - x)^2 = 0 \\
      \Rightarrow x^2 &= \vbfour + x^2 - \vbthree x \text{ or } x = \vbtwo \\
      \text{Also, }\left[\dnydxn{2}\right]_{x=\vbtwo} &= \vbfive > 0 \Rightarrow \text{ minima }
   \end{align}
   
   Hence, the required split is $\vbtwo$ and $\vbtwo$
\end{solution}
