

\question[3] Find an expression for the sum of the first $n$ terms of the series 
$1^2 + (1^2+2^2) + (1^2+2^2+3^2) + \ldots$

\insertQR{QRC}

\ifprintanswers
\fi 

\begin{solution}[\halfpage]
	\begin{align}
		S_n &= \sum_{k=1}^{n}\underbrace{\eSumOfSquares{k}}_{\text{sum of squares}} \\
		&= \dfrac{1}{6}\cdot\sum_{k=1}^{n}(2k^3+3k^2+k) = 
    \dfrac{1}{6}\cdot\left[ 2\sum_{k=1}^{n} k^3 + 3\sum_{k=1}^{n} k^2 + \sum_{k=1}^{n} k \right] \\
		&= \dfrac{1}{6}\cdot\left[ 2\cdot\eSumOfCubes{n} + 3\cdot\eSumOfSquares{n} + \eSumOfN{n}\right] \\
		&= \dfrac{n\cdot(n+1)}{12}\cdot\lbrace\underbrace{n\cdot(n+1) + 2n + 1 + 1}_{=(n+1)\cdot(n+2)}\rbrace \\
		&= \dfrac{n\cdot(n+1)^2\cdot(n+2)}{12}
	\end{align}
\end{solution}
