

\question[3] The ratio of the sum of the cubes of the terms of an infinitely decreasing 
geometric progression to the sum of the squares of its terms is 12:13. The sum of the 
first two terms of the progression is equal to $\frac{4}{3}$. Find the progression

\insertQR{QRC}

\ifprintanswers
\fi 

\begin{solution}[\halfpage]
   If $\chi = \lbrace a, ar, ar^2 \ldots\rbrace$ be the original sequence, then the sequence
   resulting from taking the cube and squares of the terms are
   
   $\chi_2 = \lbrace a^2, a^2r^2,a^2r^4 \ldots \rbrace$ and $ \chi_3 = \lbrace a^3, a^3r^3, a^3r^6 \ldots \rbrace$.
   These are themselves geometric progressions, \textit{but} with different first terms and common ratios
   
   Now, if $S_3$ be the sum of $\chi_3$ and $S_2$ the sum of $\chi_2$, then
   \begin{align}
   		\dfrac{S_3}{S_2} &= \dfrac{\frac{a^3}{1-r^3}}{\frac{a^2}{1-r^2}} = \dfrac{12}{13} \\
   		\Rightarrow \dfrac{a\cdot(1-r)\cdot(1+r)}{a\cdot(1-r)\cdot(1+r+r^2)} &= \dfrac{12}{13} \\
   		\text{ or, } \dfrac{a\cdot(1+r)}{1+r+r^2} &= \dfrac{12}{13} \\
   		\text{Also, } \underbrace{a\cdot(1+r)}_{\text{sum of first two terms}} &= \dfrac{4}{3} \\
   		\text{ And so, } \dfrac{\frac{4}{3}}{1+r+r^2} &= \dfrac{12}{13} \\
   		\Rightarrow 9r^2 + 9r - 4 &= 0 \Rightarrow r = \frac{1}{3},-\frac{4}{3}
   \end{align}
   The sequence can be infinitely decreasing \textbf{only if} $r = \frac{1}{3}$
   
   And therefore 
   \begin{align}
   	a\cdot(1+r) &= \dfrac{4}{3} \Rightarrow a = 1
   \end{align}
   Hence, the sequence is $\lbrace 1, \frac{1}{3}, \frac{1}{9}, \frac{1}{27} \ldots\rbrace$
\end{solution}
