


\ifnumequal{\value{rolldice}}{0}{
  % variables 
  \renewcommand{\vbone}{2} %p
}{
	\ifnumequal{\value{rolldice}}{1}{
		\renewcommand{\vbone}{3}
	}{
	  \ifnumequal{\value{rolldice}}{2}{
      \renewcommand{\vbone}{1}
	  }{
      \renewcommand{\vbone}{2}
	  }
	}
}

\gcalcexpr[0]\tp{\vbone * \vbone}
\gcalcexpr[0]\tq{2 * \tp}
\gcalcexpr[0]\tr{3 * \tp}
\gcalcexpr[0]\ts{\tp - 6}

\gcalcexpr[0]\af{\tp -1}
\gcalcexpr[0]\as{4*\tp - 1}
\gcalcexpr[0]\at{9*\tp - 1}
\gcalcexpr[0]\afo{16*\tp - 1}

\question[3] Find an expression for the sum of the first $n$ terms of the series 
$\af + \as + \at + \afo + \ldots$. \texttt{Hint:} Each term in the series is of the 
form $a_k = (pk-1)\cdot(qk+1),\, k \geq 1$ and $p,q \in\aleph$

\watchout

\ifprintanswers
\fi 

\begin{solution}[\halfpage]
	The $k^{th}$ term of the series is of the form $a_k = (\vbone k-1)\cdot(\vbone k+1),\, k \geq 1$
	Hence, the sum of the first $n$ terms s given by
	\begin{align}
		S_n &= \sum_{k=1}^{n}(\vbone k-1)\cdot(\vbone k+1) = \sum_{k=1}^{n}(\tp k^2-1) \\
		&= \tp\cdot\sum_{k=1}^{n}k^2 - \sum_{k=1}^{n}1 \\
		&= \tp\cdot\eSumOfSquares{n} - n \\
		&= \dfrac{n}{6}\cdot\left[\tp\cdot(2n^2 + 3n + 1) - 6\right] = \dfrac{n}{6}\left[ \tq n^2 + \tr n + \ts \right] 
	\end{align}
\end{solution}
